deps/poulet4/lib/P4automata/PreBisimulationSyntax.v
@@ -126,7 +126,13 @@ Section ConfRel.
     | _, _ => false
     end.
 
-  Definition expr_to_bit_expr (e: P4A.expr) (s: side) : bit_expr :=
+  Definition proj_state_type_ref (x: P4A.state_type a + bool) : P4A.state_ref :=
+    match x with
+    | inr b => inr b
+    | inl s => inl (proj1_sig s)
+    end.
+
+  Definition expr_to_bit_expr (s: side) (e: P4A.expr) : bit_expr :=
     match e with
     | P4A.EHdr h => BEHdr s h
     | P4A.ELit bs => BELit bs
@@ -154,18 +160,78 @@ Section ConfRel.
         (case_negated_conds cond rest)
     end.
 
-  Definition trans_cond (t: P4A.transition) (s: side) (st': P4A.state_ref) :=
+  Definition trans_cond (s: side) (t: P4A.transition) (st': P4A.state_ref) :=
     match t with
     | P4A.TGoto r =>
       if state_ref_eqb r st'
       then BRTrue
       else BRFalse
     | P4A.TSel cond cases default =>
-      let be_cond := expr_to_bit_expr cond s in
+      let be_cond := expr_to_bit_expr s cond in
       BROr (cases_cond be_cond st' cases)
            (if state_ref_eqb default st'
             then case_negated_conds be_cond cases
             else BRFalse)
     end.
+
+  Definition bit_expr_subst (s: side) (h: P4A.hdr_ref) (exp: bit_expr) (phi: bit_expr) : bit_expr.
+  Admitted.
+
+  Definition store_rel_subst (s: side) (h: P4A.hdr_ref) (exp: bit_expr) (phi: store_rel) : store_rel.
+  Admitted.
+
+  Fixpoint wp_op' (s: side) (o: P4A.op) : nat * store_rel -> nat * store_rel :=
+    fun '(buf_idx, phi) =>
+      match o with
+      | P4A.OpNil => (buf_idx, phi)
+      | P4A.OpSeq o1 o2 =>
+        wp_op' s o1 (wp_op' s o2 (buf_idx, phi))
+      | P4A.OpExtract width hdr =>
+        let new_idx := buf_idx + width - 1 in
+        let slice := BESlice (BEBuf s) new_idx buf_idx in
+        (new_idx, store_rel_subst s hdr slice phi)
+      | P4A.OpAsgn lhs rhs =>
+        (buf_idx, store_rel_subst s lhs (expr_to_bit_expr s rhs) phi)
+      end.
+
+  Definition wp_op (s: side) (o: P4A.op) (phi: store_rel) : store_rel :=
+    snd (wp_op' s o (0, phi)).
+
+  Definition preds (s: P4A.state_ref) :=
+    P4A.list_states a.
+
+  Definition pick_template (s: side) (c: conf_state) : state_template a :=
+    match s with
+    | Left => c.(cs_st1)
+    | Right => c.(cs_st2)
+    end.
+  
+  Definition wp_edge (c: conf_rel) (s: side) (st: P4A.state) : store_rel :=
+    let st' := pick_template s c.(cr_st) in
+    let tcond := trans_cond Left (P4A.st_trans st) (proj_state_type_ref st'.(st_state a)) in
+    let wp_trans := BRAnd c.(cr_rel) tcond in
+    wp_op s (P4A.st_op st) wp_trans.
+
+  Definition wp_edges (c: conf_rel) (s_left: P4A.state_type a) (s_right: P4A.state_type a) : store_rel :=
+    let state_left := P4A.find_state a s_left in
+    let state_right := P4A.find_state a s_right in
+    let c' := {| cr_st := c.(cr_st);
+                 cr_rel := wp_edge c Left state_left |} in
+    wp_edge c' Right state_right.
+
+  Definition wp_pred_pair (c: conf_rel) (preds: P4A.state_type a * P4A.state_type a) : conf_rel :=
+    let '(sl, sr) := preds in
+    {| cr_st := {| cs_st1 := {| st_state := inl sl;
+                                st_buf_len := 0 |};
+                   cs_st2 := {| st_state := inl sr;
+                                st_buf_len := 0 |} |};
+       cr_rel := wp_edges c (fst preds) (snd preds) |}.
+
+  Definition wp (c: conf_rel) : list conf_rel :=
+    let cur_st_left  := proj_state_type_ref c.(cr_st).(cs_st1).(st_state a) in
+    let cur_st_right := proj_state_type_ref c.(cr_st).(cs_st2).(st_state a) in
+    let pred_pairs := list_prod (preds cur_st_left)
+                                (preds cur_st_right) in
+    List.map (wp_pred_pair c) pred_pairs.
 
 End ConfRel.
